generate-html.sh
@@ -1,3 +1,3 @@
 #!/bin/sh
 make all
-make COQDOCFLAGS="--interpolate --title 'HJ Formalization in Coq' -l --lib-subtitles " html
+make COQDOCFLAGS="--interpolate --title 'Habanero Formalization in Coq' -l --lib-subtitles " html
